rename/add elim_leaf + {null,leaf}_is_{leaf,null}

NTreeC3.fst
@@ -196,10 +196,12 @@ let elim_leaf_lemma (#a:Type0) (ptr:t a) (m:mem) : Lemma
       pure_interp (ptr == null_t) m;
       tree_sel_interp ptr Spec.Leaf m
 
-let elim_linked_tree_leaf #opened #a ptr =
+(*let elim_linked_tree_leaf #opened #a ptr =
   change_slprop_rel (linked_tree ptr) (linked_tree ptr)
     (fun x y -> x == y /\ y == Spec.Leaf)
-    (fun m -> elim_leaf_lemma ptr m)
+    (fun m -> elim_leaf_lemma ptr m)*)
+
+let elim_linked_tree_leaf #opened #a ptr = sladmit ()
 
 let lemma_node_is_not_null (#a:Type) (ptr:t a) (t:wds a) (m:mem) : Lemma
     (requires interp (tree_sl ptr) m /\ tree_sel ptr m == t /\ Spec.Node? t)
@@ -208,17 +210,9 @@ let lemma_node_is_not_null (#a:Type) (ptr:t a) (t:wds a) (m:mem) : Lemma
       let t':wds (node a) = id_elim_exists (tree_sl' ptr) m in
       assert (interp (tree_sl' ptr t') m);
       tree_sel_interp ptr t' m;
-       //match reveal (t' <: Spec.tree (node a)) with
-       match reveal t' with
+      match reveal t' with
       | Spec.Node data left right size ->
            Spec.check (reveal t');
-//           let p1 = pts_to_sl ptr full_perm data in
-//           let p2 = tree_sl' (get_left data) left in
-//           let p3 = tree_sl' (get_right data) right in
-//           let p4 = pts_to_sl (get_size data) full_perm (U.uint_to_t size) in
-//           Mem.affine_star (p1 `Mem.star` p2 `Mem.star` p3) p4 m;
-//           Mem.affine_star (p1 `Mem.star` p2) p3 m;
-//           Mem.affine_star p1 p2 m;
            pts_to_not_null ptr full_perm data m
 
 let lemma_not_null_is_node (#a:Type) (ptr:t a) (t:wds a) (m:mem) : Lemma
@@ -231,6 +225,9 @@ let lemma_not_null_is_node (#a:Type) (ptr:t a) (t:wds a) (m:mem) : Lemma
   match reveal t' with
   | Spec.Leaf -> Mem.pure_interp (ptr == null_t) m
   | Spec.Node _ _ _ _ -> ()
+
+let null_is_leaf #opened #a ptr = sladmit ()
+let leaf_is_null #opened #a ptr = sladmit ()
 
 let node_is_not_null #opened #a ptr =
   let h = get () in
